changed wiring to use list

Connect/Wiring.v
@@ -30,100 +30,98 @@ Open Scope list_scope.
 Require Import IOModule.
 
 Module Wiring(IO:IO_SIG).
-  Inductive wiring :=
-  | base :  wiring
-  | watch_set :  wiring -> list nat -> IO.func -> nat ->  wiring
-  | just_set : wiring  -> IO.func -> nat -> wiring
-  | join : wiring -> wiring -> wiring
-  | doc : wiring -> nat -> string -> wiring.
-  Notation  "w //  m ~> f ~>  n" := (watch_set w m f n) (at level 80, m at next level) : wiring_scope. 
-  Notation  "w */  f ~>  n" := (just_set w f n) (at level 80, m at next level): wiring_scope. 
-  Notation "w1 ~&~ w2" := (join w1 w2) (at level 80) : wiring_scope.
-  Notation "w # p c " := (doc w p c) (at level 80, p at level 0) : wiring_scope.
+  Inductive component :=
+  | watch_set :   list nat -> IO.func -> nat ->  component
+  | just_set : IO.func -> nat -> component
+  | doc :  nat -> string -> component.
+  Definition wiring := list component.
+  Notation  "w //  m ~> f ~>  n" := ((watch_set m f n) :: w) (at level 80, m at next level) : wiring_scope. 
+  Notation  "w */  f ~>  n" := ((just_set f n) :: w) (at level 80, m at next level): wiring_scope. 
+  Notation "w1 ~&~ w2" := (w1 ++ w2) (at level 80) : wiring_scope.
+  Notation "w # p c " := ((doc p c)::w) (at level 80, p at level 0) : wiring_scope.
   Open Scope wiring_scope.
 
   Open Scope string_scope.
-  Fixpoint docstring' w acc :=
-    match w with
-      | base  => acc
-      | watch_set w' from fn to => docstring' w' acc
-      | just_set w' fn to =>docstring' w' acc
-      | join w1 w2 => docstring' w2 (docstring' w1 acc)
-      | doc w' p c =>
-        let n : string := (String (ascii_of_nat p) "") in 
-        docstring' w' ("Port Ascii(" ++ n ++ ") "++c ++ "\n" ++ acc)
-
+  Fixpoint docstring' l acc :=
+    match l with
+      | [] => acc
+      | w::w' => 
+        match w with
+          | watch_set from fn to => docstring' w' acc
+          | just_set  fn to =>docstring' w' acc
+          | doc  p c =>
+            let n : string := (String (ascii_of_nat p) "") in 
+            docstring' w' ("Port Ascii(" ++ n ++ ") "++c ++ "\n" ++ acc)
+        end
     end.
   Definition docstring w := docstring' w "".
-  Fixpoint output_pins w s: set nat :=
+  Fixpoint output_pins l s: set nat :=
     let add_i := set_add%nat nat eq_nat_dec in
+    match l with
+      | [] => s
+      | w::w' =>
     match w with 
-      | base  =>
-        s
-      | watch_set w' from fn to =>
+      | watch_set  from fn to =>
         output_pins w' (add_i  to s)
-      | just_set w' fn to =>
+      | just_set  fn to =>
         output_pins w' (add_i to s)
-      | join w1 w2 => set_union%nat nat eq_nat_dec (output_pins w1 s) (output_pins w2 nil)
-      | doc w' _ _ =>  output_pins w' s
+      | doc _ _ =>  output_pins w' s
+    end
     end.
 
-  Fixpoint input_pins w s: set nat :=
+  Fixpoint input_pins l s: set nat :=
     let add_i := set_add%nat nat eq_nat_dec in
-    match w with 
-      | base  => s
-      | watch_set w' from fn to =>
-        output_pins w'
-                    (fold_left (fun se f => add_i f se) s  from)
+    match l with
+      | [] => s
+      | w::w' =>
+        match w with 
+          | watch_set  from fn to =>
+            output_pins w'
+                        (fold_left (fun se f => add_i f se) s  from)
 
-      | just_set w' fn to =>  output_pins w' s
-      | join w1 w2 => set_union%nat nat eq_nat_dec (output_pins w1 s) (output_pins w2 nil)
-      | doc w' _ _ =>  input_pins w' s
+          | just_set  fn to =>  output_pins w' s
+          | doc  _ _ =>  input_pins w' s
+        end
     end.
 
-  Fixpoint all_pins' w s: set nat :=
+  Fixpoint all_pins' l s: set nat :=
     let add_i := set_add%nat nat eq_nat_dec in
+    match l with
+      | [] => s
+      | w::w' =>
     match w with 
-      | base  => s
-      | watch_set w' from fn to =>
+      | watch_set  from fn to =>
         all_pins' w'
                   (add_i to (fold_left (fun se f => add_i f se) s  from))
 
-      | just_set w' fn to =>  all_pins' w' (add_i to s)
-      | join w1 w2 => set_union%nat nat eq_nat_dec (all_pins' w1 s) (all_pins' w2 nil)
-      | doc w' _ _ =>  all_pins' w' s
+      | just_set  fn to =>  all_pins' w' (add_i to s)
+      | doc  _ _ =>  all_pins' w' s
+                               end
     end.
   Definition pins w := all_pins' w nil.
   (* Checks that all observers have a source and that only one setter per nat *)
-  Fixpoint valid_wiring' w ins outs: Prop :=
+  Fixpoint valid_wiring' l ins outs: Prop :=
     let add_i := set_add%nat nat eq_nat_dec in
     let notin := (fun el  s => (not (set_In%nat nat  el s))) in
     let union := set_union%nat nat eq_nat_dec in
     let intersect := set_inter%nat nat eq_nat_dec in
-    match w with 
-      | base  =>
+    match l with
+      | [] =>
         (* Check that the intersection of inputs and outputs is inputs,
          ie, everything can be read *)
         (intersect ins outs) = ins
-      | watch_set w' from fn to =>
+      | w::w' =>
+    match w with 
+      | watch_set  from fn to =>
         notin to outs /\
         IO.nargs fn = length from /\
         valid_wiring' w'
                       ( fold_left  (fun s f => add_i f s) ins from) (add_i to outs)
-      | just_set w' fn to=>
+      | just_set  fn to=>
         notin to outs
         /\ valid_wiring' w' ins (add_i to outs)
-      | join w1 w2 =>
-        let w1_out := output_pins w1 [] in
-        let w2_out := output_pins w2 [] in
-        (* intersect w1_out w2_out = [] /\ (*is implicitly checked*)  *) 
-        (* We union in the others outputs to say that w2 is promising
-        that it will make this available as an output (so treat it as an
-        available input too *)
-        valid_wiring' w1 (union w2_out ins) (union
-                                               w2_out outs) /\
-        valid_wiring' w2  (union w1_out ins) (union w1_out outs)
-      | doc w' _ _ =>  valid_wiring' w'  ins outs
+      | doc  _ _ =>  valid_wiring' w'  ins outs
+                                   end
     end.
   Definition valid_wiring w : Prop :=
     valid_wiring' w nil nil.
@@ -136,34 +134,35 @@ Module Wiring(IO:IO_SIG).
     repeat (try split; try omega).
 
   (* Rewire w1 so it won't interfere with w2 *)
-  Fixpoint rewire_offset w1 n: wiring :=
+  Definition wire_add_offset n w1: component :=
     match w1 with
-      | base => base
-      | watch_set w' from fn to =>
-        (watch_set  (rewire_offset w' n) (map (fun x=>x+ n)from) fn (to+n))
-      | just_set w' fn to =>
-        just_set  (rewire_offset w' n) fn (to+n) 
-      | join w1 w2 =>
-        join (rewire_offset w1 n) ( rewire_offset w2 n ) 
-      | doc w' p c =>  
-        (doc  (rewire_offset w' n ) (p+n) c)
+      | watch_set  from fn to =>
+        (watch_set   (map (fun x=>x+ n)from) fn (to+n))
+      | just_set  fn to =>
+        just_set fn (to+n) 
+      | doc  p c =>  
+        doc   (p+n) c
     end.
-  Definition rewire w1 w2 : wiring :=
+  Definition rewire w1 w2 :wiring :=
     let m := fold_left max (pins w2) 0 in
-    rewire_offset w1 (m+1).
+    map (wire_add_offset (m+1)) w1.
 
   Theorem rewire_safe : forall w w',
                           valid_wiring w ->
                           valid_wiring w' ->
                           valid_wiring (rewire w w' ~&~ w').
     intros.
+    induction w.
+    auto.
+    unfold rewire.
+    assert (H1:forall (A B: Type) (a:A) (b:list A) (f: A-> B) f, map f (a::b) = (f a) :: (@map A B  f b)).
+    intros.
+    auto.
+    rewrite H1; auto.
+
+    remember (wire_add_offset ((fold_left max (pins w') 0)+1)) as f.
     unfold valid_wiring.
     unfold valid_wiring'.
-    simpl.
-    fold valid_wiring'.
-    fold valid_wiring.
-    split.
-    admit.
     admit.
   Qed.
 End Wiring.
